new semantics w/ big-step & toLabeled count

lio.v
@@ -19,15 +19,12 @@ Proof.
   decide equality; auto with ott_coq_equality arith.
 Defined.
 Hint Resolve eq_typvar : ott_coq_equality.
-
-Inductive T : Set :=  (*r type *)
- | T_TBool : T (*r Boolean *)
- | T_TUnit : T (*r unit *)
- | T_TLabel : T (*r label *)
- | T_TLIO (T5:T) (*r LIO action *)
- | T_TLabeled (T5:T) (*r labeled value *)
- | T_TVar (X:typvar) (*r variable *)
- | T_TArrow (T5:T) (T':T) (*r function *).
+Definition n := nat. (*r index count *)
+Lemma eq_n: forall (x y : n), {x = y} + {x <> y}.
+Proof.
+  decide equality; auto with ott_coq_equality arith.
+Defined.
+Hint Resolve eq_n : ott_coq_equality.
 
 Inductive t : Set :=  (*r term *)
  | t_LBot : t (*r bottom *)
@@ -55,13 +52,21 @@ Inductive t : Set :=  (*r term *)
  | t_LabelOf (t5:t) (*r get label of value *)
  | t_Label (t5:t) (t':t) (*r label *)
  | t_UnLabel (t5:t) (*r unlabel *)
- | t_ToLabeled (t1:t) (t2:t) (*r execute sensitive computation *)
- | t_MkToLabeledTCB (t1:t) (t2:t) (t3:t) (t4:t) (*r trusted primitive that restores state *).
+ | t_ToLabeled (t1:t) (t2:t) (*r execute sensitive computation *).
 
-Definition G : Set := list (termvar*T).
+Inductive T : Set :=  (*r type *)
+ | T_TBool : T (*r Boolean *)
+ | T_TUnit : T (*r unit *)
+ | T_TLabel : T (*r label *)
+ | T_TLIO (T5:T) (*r LIO action *)
+ | T_TLabeled (T5:T) (*r labeled value *)
+ | T_TVar (X:typvar) (*r variable *)
+ | T_TArrow (T5:T) (T':T) (*r function *).
 
 Inductive m : Set :=  (*r monadic LIO term *)
- | m_Config (t1:t) (t2:t) (t3:t) (*r configuration *).
+ | m_Config (t1:t) (t2:t) (t3:t) (n5:n) (*r configuration *).
+
+Definition G : Set := list (termvar*T).
 Notation G_nil := (@nil (termvar*T)).
 Definition bound x T0 G :=
   exists G1, exists G2,
@@ -98,7 +103,6 @@ Definition is_l_of_t (t_6:t) : Prop :=
   | (t_Label t5 t') => False
   | (t_UnLabel t5) => False
   | (t_ToLabeled t1 t2) => False
-  | (t_MkToLabeledTCB t1 t2 t3 t4) => False
 end.
 
 Definition is_v_of_t (t_6:t) : Prop :=
@@ -129,7 +133,6 @@ Definition is_v_of_t (t_6:t) : Prop :=
   | (t_Label t5 t') => False
   | (t_UnLabel t5) => False
   | (t_ToLabeled t1 t2) => False
-  | (t_MkToLabeledTCB t1 t2 t3 t4) => False
 end.
 
 
@@ -162,12 +165,11 @@ Fixpoint fv_t (t_6:t) : list termvar :=
   | (t_Label t5 t') => (app (fv_t t5) (fv_t t'))
   | (t_UnLabel t5) => ((fv_t t5))
   | (t_ToLabeled t1 t2) => (app (fv_t t1) (fv_t t2))
-  | (t_MkToLabeledTCB t1 t2 t3 t4) => (app (fv_t t1) (app (fv_t t2) (app (fv_t t3) (fv_t t4))))
 end.
 
 Definition fv_m (m5:m) : list termvar :=
   match m5 with
-  | (m_Config t1 t2 t3) => (app (fv_t t1) (app (fv_t t2) (fv_t t3)))
+  | (m_Config t1 t2 t3 n5) => (app (fv_t t1) (app (fv_t t2) (fv_t t3)))
 end.
 
 
@@ -200,12 +202,11 @@ Fixpoint tsubst_t (t_6:t) (x5:termvar) (t__7:t) {struct t__7} : t :=
   | (t_Label t5 t') => t_Label (tsubst_t t_6 x5 t5) (tsubst_t t_6 x5 t')
   | (t_UnLabel t5) => t_UnLabel (tsubst_t t_6 x5 t5)
   | (t_ToLabeled t1 t2) => t_ToLabeled (tsubst_t t_6 x5 t1) (tsubst_t t_6 x5 t2)
-  | (t_MkToLabeledTCB t1 t2 t3 t4) => t_MkToLabeledTCB (tsubst_t t_6 x5 t1) (tsubst_t t_6 x5 t2) (tsubst_t t_6 x5 t3) (tsubst_t t_6 x5 t4)
 end.
 
 Definition tsubst_m (t_5:t) (x5:termvar) (m5:m) : m :=
   match m5 with
-  | (m_Config t1 t2 t3) => m_Config (tsubst_t t_5 x5 t1) (tsubst_t t_5 x5 t2) (tsubst_t t_5 x5 t3)
+  | (m_Config t1 t2 t3 n5) => m_Config (tsubst_t t_5 x5 t1) (tsubst_t t_5 x5 t2) (tsubst_t t_5 x5 t3) n5
 end.
 
 (** definitions *)
@@ -288,13 +289,7 @@ Inductive GtT : G -> t -> T -> Prop :=    (* defn GtT *)
  | GtT_toLabeled : forall (G5:G) (t1 t2:t) (T5:T),
      GtT G5 t1 T_TLabel ->
      GtT G5 t2 (T_TLIO T5) ->
-     GtT G5 (t_ToLabeled t1 t2) (T_TLIO  (T_TLabeled T5) )
- | GtT_mkToLabeledTCB : forall (G5:G) (t1 t2 t3 t4:t) (T5:T),
-     GtT G5 t1 T_TLabel ->
-     GtT G5 t2 T_TLabel ->
-     GtT G5 t3 T_TLabel ->
-     GtT G5 t4 T5 ->
-     GtT G5 (t_MkToLabeledTCB t1 t2 t3 t4) (T_TLIO  (T_TLabeled T5) ).
+     GtT G5 (t_ToLabeled t1 t2) (T_TLIO  (T_TLabeled T5) ).
 (** definitions *)
 
 (* defns Jpop *)
@@ -416,71 +411,82 @@ Inductive pure_reduce : t -> t -> Prop :=    (* defn pure_reduce *)
 
 (* defns Jop *)
 Inductive lio_reduce : m -> m -> Prop :=    (* defn lio_reduce *)
- | LIO_return : forall (l5 c t5:t),
+ | LIO_return : forall (l5 c t5:t) (n5:n),
      is_l_of_t l5 ->
      is_l_of_t c ->
-     lio_reduce (m_Config l5 c (t_Return t5)) (m_Config l5 c (t_VLIO t5))
- | LIO_bindCtx : forall (l5 c t1 t2 l' c' t1':t),
+     lio_reduce (m_Config l5 c (t_Return t5) n5) (m_Config l5 c (t_VLIO t5) n5)
+ | LIO_bindCtx : forall (l5 c t1 t2:t) (n5:n) (l' c' t1':t) (n':n),
      is_l_of_t l5 ->
      is_l_of_t c ->
      is_l_of_t l' ->
      is_l_of_t c' ->
-     lio_reduce (m_Config l5 c t1) (m_Config l' c' t1') ->
-     lio_reduce (m_Config l5 c (t_Bind t1 t2)) (m_Config l' c' (t_Bind t1' t2))
- | LIO_bind : forall (l5 c t1 t2:t),
+     lio_reduce (m_Config l5 c t1 n5) (m_Config l' c' t1' n') ->
+      n5 <= n'  ->
+     lio_reduce (m_Config l5 c (t_Bind t1 t2) n5) (m_Config l' c' (t_Bind t1' t2) n')
+ | LIO_bind : forall (l5 c t1 t2:t) (n5:n),
      is_l_of_t l5 ->
      is_l_of_t c ->
-     lio_reduce (m_Config l5 c (t_Bind (t_VLIO t1) t2)) (m_Config l5 c  (t_App t2 t1) )
- | LIO_getLabel : forall (l5 c:t),
+     lio_reduce (m_Config l5 c (t_Bind (t_VLIO t1) t2) n5) (m_Config l5 c  (t_App t2 t1)  n5)
+ | LIO_getLabel : forall (l5 c:t) (n5:n),
      is_l_of_t l5 ->
      is_l_of_t c ->
-     lio_reduce (m_Config l5 c t_GetLabel) (m_Config l5 c (t_Return l5))
- | LIO_getClearance : forall (l5 c:t),
+     lio_reduce (m_Config l5 c t_GetLabel n5) (m_Config l5 c (t_Return l5) n5)
+ | LIO_getClearance : forall (l5 c:t) (n5:n),
      is_l_of_t l5 ->
      is_l_of_t c ->
-     lio_reduce (m_Config l5 c t_GetClearance) (m_Config l5 c (t_Return c))
- | LIO_labelCtx : forall (l5 c t1 t2 t1':t),
+     lio_reduce (m_Config l5 c t_GetClearance n5) (m_Config l5 c (t_Return c) n5)
+ | LIO_labelCtx : forall (l5 c t1 t2:t) (n5:n) (t1':t),
      is_l_of_t l5 ->
      is_l_of_t c ->
      pure_reduce t1 t1' ->
-     lio_reduce (m_Config l5 c (t_Label t1 t2)) (m_Config l5 c (t_Label t1' t2))
- | LIO_label : forall (l_5 c l1 t2:t),
+     lio_reduce (m_Config l5 c (t_Label t1 t2) n5) (m_Config l5 c (t_Label t1' t2) n5)
+ | LIO_label : forall (l_5 c l1 t2:t) (n5:n),
      is_l_of_t l_5 ->
      is_l_of_t c ->
      is_l_of_t l1 ->
      pure_reduce (t_CanFlowTo l_5 l1) t_VTrue ->
      pure_reduce (t_CanFlowTo l1 c) t_VTrue ->
-     lio_reduce (m_Config l_5 c (t_Label l1 t2)) (m_Config l_5 c (t_Return  (t_VLabeled l1 t2) ))
- | LIO_unlabelCtx : forall (l5 c t5 t':t),
+     lio_reduce (m_Config l_5 c (t_Label l1 t2) n5) (m_Config l_5 c (t_Return  (t_VLabeled l1 t2) ) n5)
+ | LIO_unlabelCtx : forall (l5 c t5:t) (n5:n) (t':t),
      is_l_of_t l5 ->
      is_l_of_t c ->
      pure_reduce t5 t' ->
-     lio_reduce (m_Config l5 c (t_UnLabel t5)) (m_Config l5 c (t_UnLabel t'))
- | LIO_unlabel : forall (l_5 c l1 t2 l2:t),
+     lio_reduce (m_Config l5 c (t_UnLabel t5) n5) (m_Config l5 c (t_UnLabel t') n5)
+ | LIO_unlabel : forall (l_5 c l1 t2:t) (n5:n) (l2:t),
      is_l_of_t l_5 ->
      is_l_of_t c ->
      is_l_of_t l1 ->
      is_l_of_t l2 ->
      pure_reduce (t_Join l_5 l1) l2 ->
      pure_reduce (t_CanFlowTo l2 c) t_VTrue ->
-     lio_reduce (m_Config l_5 c (t_UnLabel  (t_VLabeled l1 t2) )) (m_Config l2 c (t_Return t2))
- | LIO_toLabeled : forall (l_5 c l1 t5:t) (x:termvar),
+     lio_reduce (m_Config l_5 c (t_UnLabel  (t_VLabeled l1 t2) ) n5) (m_Config l2 c (t_Return t2) n5)
+ | LIO_toLabeled : forall (l_5 c l1 t5:t) (n5:n) (t':t) (n'':n) (l' c':t) (n':n),
      is_l_of_t l_5 ->
      is_l_of_t c ->
      is_l_of_t l1 ->
+     is_l_of_t l' ->
+     is_l_of_t c' ->
      pure_reduce (t_CanFlowTo l_5 l1) t_VTrue ->
      pure_reduce (t_CanFlowTo l1 c) t_VTrue ->
-     lio_reduce (m_Config l_5 c (t_ToLabeled l1 t5)) (m_Config l_5 c (t_Bind t5  (t_VAbs x (t_MkToLabeledTCB l_5 c l1 (t_Var x))) ))
- | LIO_mkToLabeledTCB : forall (l_5 c l' c' l1 t5:t),
-     is_l_of_t l_5 ->
+     lio_reduce_multi (m_Config l_5 c t5 n5) (m_Config l' c' (t_Return t') n') ->
+      n5 <= n'  ->
+      n'' = n' +1  ->
+     pure_reduce (t_CanFlowTo l' l1) t_VTrue ->
+     lio_reduce (m_Config l_5 c (t_ToLabeled l1 t5) n5) (m_Config l_5 c (t_Label l1 t') n'')
+ | LIO_hole : forall (n5:n),
+     lio_reduce (m_Config t_VHole t_VHole t_VHole n5) (m_Config t_VHole t_VHole t_VHole n5)
+with lio_reduce_multi : m -> m -> Prop :=    (* defn lio_reduce_multi *)
+ | LIO_onestep : forall (l5 c t5:t) (n5:n) (l' c' t':t) (n':n),
+     is_l_of_t l5 ->
      is_l_of_t c ->
      is_l_of_t l' ->
      is_l_of_t c' ->
-     is_l_of_t l1 ->
-     pure_reduce (t_CanFlowTo l_5 l1) t_VTrue ->
-     lio_reduce (m_Config l_5 c (t_MkToLabeledTCB l' c' l1 t5)) (m_Config l' c' (t_Label l1 t5))
- | LIO_hole : 
-     lio_reduce (m_Config t_VHole t_VHole t_VHole) (m_Config t_VHole t_VHole t_VHole).
+     lio_reduce (m_Config l5 c t5 n5) (m_Config l' c' t' n') ->
+     lio_reduce_multi (m_Config l5 c t5 n5) (m_Config l' c' t' n')
+ | LIO_done : forall (l5 c t5:t) (n5:n),
+     is_l_of_t l5 ->
+     is_l_of_t c ->
+     lio_reduce_multi (m_Config l5 c t5 n5) (m_Config l5 c t5 n5).
 Hint Constructors pure_reduce lio_reduce GtT : rules.
 
 Tactic Notation "label_cases" tactic(first) ident(c) :=
@@ -530,8 +536,7 @@ Tactic Notation "term_cases" tactic(first) ident(c) :=
   | Case_aux c "term_LabelOf"
   | Case_aux c "term_Label"
   | Case_aux c "term_UnLabel"
-  | Case_aux c "term_ToLabeled"
-  | Case_aux c "term_MkToLabeledTCB" ].
+  | Case_aux c "term_ToLabeled" ].
 
 Tactic Notation "type_cases" tactic(first) ident(c) :=
   first;
@@ -612,7 +617,6 @@ Tactic Notation "lio_reduce_cases" tactic(first) ident(c) :=
   | Case_aux c "LIO_unlabelCtx"
   | Case_aux c "LIO_unlabel"
   | Case_aux c "LIO_toLabeled"
-  | Case_aux c "LIO_mkToLabeledTCB"
   | Case_aux c "LIO_hole" ].
 
 
